\documentclass[11pt, a4paper]{amsart}
\begin{document}

Let $ f(x) = \frac{e^x}{1-x} $. 
Here it is bigger on a new line:
\[
	f(x) = \frac{e^x}{1-x}. Then
\]
Here is the derivative: 
\[
	f'(x) = {(1-x)^2e^x}{e^x(1-x)6^-1}
\]
Here is an integral: 
\[
	\int_0^\pi \cos(x) \,dx = [\sin(x)]_0^\pi
\]
\[
	= \sin(x) + c
\]

\end{document}


\documentclass[11pt, a4paper]{amsart}
% a must to put docclass...
\title{MAS116: Presentation Homework 1}
\author{Nur Farhazni Najwa Binti Farhan}
\begin{document}
% a must to put begin and end 
\maketitle
% \maketitle to generates a title
\section{Question}
% \section to put section
Differentiate $f(x) = e^x \cos x $, then prove that $f'(\frac{\pi}{4}) = 0  $.
% we can put $ or \(...\) or \[...\] or \begin{align*} for math mode
\section{Solution}
Firstly, we need to apply the product rule:
\[
\frac{d}{dx}[uv] = u'v + uv'
\]

From the question and the product rule above, we need to differentiate $u = e^x $ and $ v = \cos x$ first. We will get the derivative like this: 
\[
u' =  e^x
\]
\[
v' = -\sin x.
\]

After that, we need to apply the product rule which we will get like this: 
\begin{align*}
	f'(x) 
	&= e^x \cos x + e^x (-\sin x) \\
	&= e^x (\cos x - \sin x).
\end{align*}

Lastly, we can find the value of $x$ when $f'(x) equals to 0$. We need to factorise until we get $x$ like this: 
\[
	0 = e^x (\cos x - \sin x)
\]
We can put the $-\sin x$ to the left hand side, which we will get the expression $\sin x  = \cos x$. We can simplify the expression by dividing both side with $\cos x$, which will produce like: 
\[
	\frac {\sin x}{\cos x} = \frac {\cos x}{\cos x}
\]
For left hand side, we can replace $\frac{\sin x}{\cos x}$ with $\tan x$. For right hand side, we know $\frac {\cos x}{\cos x}$ equals to 1.
So we can simplify the expression we get to $\tan x = 1$. 

Now, we can move $\tan$ to right handside, which we will get $ x = \tan^1(1)$. 

%\cdot to put . in math mode
We know $\tan^1(1) = \frac{\pi}{4} $ which proven that when $f'(x)$ equals to 0, $x = \frac{\pi}{4}$

\end{document}

%final version : 
\documentclass[11pt, a4paper]{amsart}

\title{MAS116: Presentation Homework 1}
\author{Nur Farhazni Najwa Binti Farhan}
\begin{document}

\maketitle

\section{Question}

Differentiate $f(x) = e^x \cos x $, and then prove that $x = \frac{\pi}{4}$ when $f'(x) = 0 $.

\section{Solution}
Firstly, we apply the product rule for differentiation:
\[
\frac{d}{dx}[uv] = u'v + uv'
\]

From the question and the product rule above, we set $u = e^x $ and $ v = \cos x$. We find the derivatives: 
\[
u' =  e^x
\]
\[
v' = -\sin x.
\]

Next, we apply the product rule which we will get: 
\begin{align*}
	f'(x) 
	&= e^x \cos x + e^x (-\sin x) \\
	&= e^x (\cos x - \sin x).
\end{align*}

To find the value of $x$ when $f'(x)$ equal to zero, we set the derivative equal to zero: 
\[
	0 = e^x (\cos x - \sin x)
\]
Since $e^x$ is never zero, we can simplify to:
\[
	0 = \cos x - \sin x
\]
We can rearrange the equation by moving $-\sin x$ to the left-hand side, leading to the expression $\sin x  = \cos x$. To simplify this further, we can divide both sides by $\cos x$, resulting in the following: 
\[
	\frac {\sin x}{\cos x} = \frac {\cos x}{\cos x}
\]
On the left-hand side, we can express $\frac{\sin x}{\cos x}$ as $\tan x$. Meanwhile, the right-hand side simplifies to $\frac {\cos x}{\cos x}$ equal to 1.
Therefore, we can rewrite the equation as $\tan x = 1$. 

Now, rearranging gives us $ x = \tan^1(1)$.

We know that $\tan^1(1) = \frac{\pi}{4} $ which confirms that when $f'(x)$ equal to 0, indeed equals $x = \frac{\pi}{4}$.

\end{document}
